Makefile
@@ -1,18 +1,18 @@
-all: lngen ott
+all: lngen ott coq
 
-coq: Exp/Exp_ott.v Exp/Exp_inf.v
-	coqc Exp/Exp_ott.v
-	coqc Exp/Exp_inf.v
+coq: Exp_ott.v Exp_inf.v
+	coqc Exp_ott.v
+	coqc Exp_inf.v
 
 Exp_inf.v: lngen
 lngen: Exp.ott
-	lngen --coq Exp/Exp_inf.v Exp.ott
+	lngen --coq Exp_inf.v Exp.ott --coq-ott Exp_ott
 
 Exp_all.tex: ott
 Exp_ott.v: ott
 ott: Exp.ott
-	ott -i Exp.ott -o Exp/Exp_all.tex -o Exp/Exp_ott.v
+	ott -i Exp.ott -o Exp_all.tex -o Exp_ott.v
 
 .PHONY:
 clean:
-	cd Exp && rm *.aux *.vo *.vok *.vos *.glob
+	rm *.aux *.vo *.vok *.vos *.glob
